Lp2lc/Next/STLC/package.lean
@@ -1,4 +1,0 @@
-import «Lp2lc».Next.STLC.STLCDef
-import «Lp2lc».Next.STLC.__Infer
-import «Lp2lc».Next.STLC.__Infer_Umbral
-import «Lp2lc».Next.STLC.Proof
